Fixing ILN for mutual.

IL/ILN.v
@@ -2,15 +2,16 @@ Require Import List.
 Require Export Util Var Val Exp Env Map CSet AutoIndTac IL Bisim Infra.Status Pos.
 
 Set Implicit Arguments.
+Unset Printing Records.
 
 Inductive nstmt : Type :=
 | nstmtLet    (x : var) (e: exp) (s : nstmt)
 | nstmtIf     (e : exp) (s : nstmt) (t : nstmt)
-| nstmtApp   (l : lab) (Y:args)
+| nstmtApp   (l : var) (Y:args)
 | nstmtReturn (e : exp)
 | nstmtExtern (x : var) (f:external) (Y:args) (s:nstmt)
 (* block f Z : rt = s in b *)
-| nstmtFun    (l : lab) (Z:params) (s : nstmt) (t : nstmt).
+| nstmtFun    (F : list (var * params * nstmt)) (t : nstmt).
 
 Fixpoint freeVars (s:nstmt) : set var :=
   match s with
@@ -19,7 +20,9 @@ Fixpoint freeVars (s:nstmt) : set var :=
     | nstmtApp l Y => list_union (List.map Exp.freeVars Y)
     | nstmtReturn e => Exp.freeVars e
     | nstmtExtern x f Y s => (freeVars s \ {{x}}) ∪ list_union (List.map Exp.freeVars Y)
-    | nstmtFun l Z s1 s2 => (freeVars s1 \ of_list Z) ∪ freeVars s2
+    | nstmtFun F s2 =>
+      list_union (List.map (fun f => (freeVars (snd f) \ of_list (snd (fst f)))) F)
+                 ∪ freeVars s2
   end.
 
 (** *** Functional Semantics *)
@@ -29,11 +32,19 @@ Module F.
     blockI {
         block_L : onv block;
         block_E : onv val;
-        block_F : lab * params * nstmt
+        block_F : list (var * params * nstmt);
+        block_f : nat
       }.
 
   Definition labenv := onv block.
   Definition state : Type := (labenv * onv val * nstmt)%type.
+
+  Definition mkBlock L E F f (_:var * params * nstmt) :=
+    blockI L E F f.
+
+  Definition mkBlocks L E F :=
+    mapi (mkBlock L E F) F.
+
 
   Inductive step : state -> event -> state -> Prop :=
   | nstepExp L E x e b v
@@ -53,20 +64,21 @@ Module F.
     : step (L, E, nstmtIf e b1 b2) EvtTau (L, E, b2)
 
 
-  | nstepGoto (L:labenv) (E:onv val) (l l':lab) Y Z (s:nstmt) L' E'
+  | nstepGoto L E l l' Y Z s L' E' F f
     (len:length Z = length Y)
     (lEQ:l = l') (* hack: otherwise inversions confuse guardedness checker in
                   simulation proofs*)
 
-    (Ldef:L (counted l) = Some (blockI L' E' (l',Z,s))) E'' vl
+    (Ldef:L l = Some (blockI L' E' F f)) E'' vl
     (def:omap (exp_eval E) Y = Some vl)
+    (sdef : get F f (l', Z, s))
     (updOk:E'[Z <-- List.map Some vl]  = E'')
     : step (L, E, nstmtApp l Y)
            EvtTau
-           (L'[(counted l) <- Some (blockI L' E' (l,Z,s))], E'', s)
+           (L'[List.map (fst ∘ fst) F <-- List.map Some (mkBlocks L' E' F)], E'', s)
 
-  | stepLet L E f s Z t
-    : step (L, E, nstmtFun f Z s t) EvtTau (L[counted f <- Some (blockI L E (f,Z,s))], E, t)
+  | stepLet (L:onv block) E F t
+    : step (L, E, nstmtFun F t) EvtTau (L[List.map (fst ∘ fst) F <-- List.map Some (mkBlocks L E F)], E, t)
 
   | stepExtern L E x f Y s vl v
     (def:omap (exp_eval E) Y = Some vl)
@@ -79,6 +91,7 @@ Module F.
     internally_deterministic step.
   Proof.
     hnf; intros. inv H; inv H0; split; eauto; try congruence.
+    rewrite Ldef0 in Ldef. inv Ldef. repeat (get_functional; subst); congruence.
   Qed.
 
   Lemma step_dec
@@ -90,12 +103,17 @@ Module F.
     - case_eq (exp_eval V e); intros.
       left. case_eq (val2bool v); intros; eexists EvtTau; eauto using step.
       right. stuck.
-    - case_eq (L (counted l)); intros.
-      + destruct b as [? ? [[? ?] ?]].
-        decide (l = l0); subst; try now (right; stuck).
-        decide (length l1 = length Y); try now (right; stuck).
-        case_eq (omap (exp_eval V) Y); intros; try now (right; stuck).
-        left. eexists EvtTau. econstructor. econstructor; eauto.
+    - case_eq (L l); intros.
+      + destruct b as [L' E' F' f'].
+        destruct (get_dec F' f') as [[[[l' Z] s] ?]|].
+        * decide (l = l'); subst; try now (right; stuck2).
+          decide (length Z = length Y); try now (right; stuck2).
+          case_eq (omap (exp_eval V) Y); intros; try now (right; stuck2).
+          left. eexists EvtTau. econstructor. econstructor; eauto.
+          orewrite (l' + 0=l'). eauto.
+          right; stuck2. rewrite Ldef in H. inv H. get_functional; subst. congruence.
+          right; stuck2. rewrite Ldef in H. inv H. get_functional; subst. congruence.
+        * right; stuck2. rewrite Ldef in H. inv H. eauto.
       + right. stuck.
     - right. stuck.
     - case_eq (omap (exp_eval V) Y); intros; try now (right; stuck).
@@ -112,12 +130,20 @@ Module I.
   Inductive block : Type :=
     blockI {
         block_L : onv block;
-        block_F : lab * params * nstmt
+        block_F : list (var * params * nstmt);
+        block_f : nat
       }.
 
   Definition labenv := onv block.
   Definition state : Type := (labenv * onv val * nstmt)%type.
   Definition labenv_empty : labenv := fun _ => None.
+
+  Definition mkBlock L F f (_:var *params*nstmt):=
+    blockI L F f.
+
+  Definition mkBlocks L F :=
+    mapi (mkBlock L F) F.
+
 
   Inductive step : state -> event -> state -> Prop :=
   | nstepExp L E x e b v
@@ -136,20 +162,23 @@ Module I.
     (condFalse:val2bool v = false)
     : step (L, E, nstmtIf e b1 b2) EvtTau (L, E, b2)
 
-  | nstepGoto (L:labenv) (E:onv val) (l l':lab) Y Z (s:nstmt) L' vl
+  | nstepGoto L E l l' Y Z s L' F f
     (len:length Z = length Y)
-    (lEQ: l = l')
-    (Ldef:L (counted l) = Some (blockI L' (l',Z,s))) E''
+    (lEQ:l = l') (* hack: otherwise inversions confuse guardedness checker in
+                  simulation proofs*)
+
+    (Ldef:L l = Some (blockI L' F f)) E'' vl
     (def:omap (exp_eval E) Y = Some vl)
-    (updOk:E [Z <-- List.map Some vl]  = E'')
+    (sdef : get F f (l', Z, s))
+    (updOk:E[Z <-- List.map Some vl]  = E'')
     : step (L, E, nstmtApp l Y)
            EvtTau
-           (L'[(counted l) <- Some (blockI L' (l,Z,s))], E'', s)
+           (L'[List.map (fst ∘ fst) F <-- List.map Some (mkBlocks L F)], E'', s)
 
-  | stepLet L E f s Z t
-    : step (L, E, nstmtFun f Z s t)
+  | stepLet L E F t
+    : step (L, E, nstmtFun F t)
            EvtTau
-           (L[counted f <- Some (blockI L (f,Z,s))], E, t)
+           (L[List.map (fst ∘ fst) F <-- List.map Some (mkBlocks L F)], E, t)
 
   | stepExtern L E x f Y s vl v
     (def:omap (exp_eval E) Y = Some vl)
@@ -162,6 +191,7 @@ Module I.
     internally_deterministic step.
   Proof.
     hnf; intros. inv H; inv H0; split; eauto; try congruence.
+    rewrite Ldef0 in Ldef. inv Ldef. get_functional; subst. congruence.
   Qed.
 
   Lemma step_externally_determined
@@ -169,24 +199,30 @@ Module I.
   Proof.
     hnf; intros.
     inv H; inv H0; eauto; try get_functional; try congruence.
+    rewrite Ldef0 in Ldef. inv Ldef. get_functional; subst. congruence.
   Qed.
 
 
   Lemma step_dec
   : reddec step.
   Proof.
-    hnf; intros. destruct x as [[L V] []].
+      hnf; intros. destruct x as [[L V] []].
     - case_eq (exp_eval V e); intros. left. eexists EvtTau; eauto using step.
       right. stuck.
     - case_eq (exp_eval V e); intros.
       left. case_eq (val2bool v); intros; eexists EvtTau; eauto using step.
       right. stuck.
-    - case_eq (L (counted l)); intros.
-      + destruct b as [? [[? ?] ?]].
-        decide (l = l0); subst; try now (right; stuck).
-        decide (length l1 = length Y); try now (right; stuck).
-        case_eq (omap (exp_eval V) Y); intros; try now (right; stuck).
-        left. eexists EvtTau. econstructor. econstructor; eauto.
+    - case_eq (L l); intros.
+      + destruct b as [L' F' f'].
+        destruct (get_dec F' f') as [[[[l' Z] s] ?]|].
+        * decide (l = l'); subst; try now (right; stuck2).
+          decide (length Z = length Y); try now (right; stuck2).
+          case_eq (omap (exp_eval V) Y); intros; try now (right; stuck2).
+          left. eexists EvtTau. econstructor. econstructor; eauto.
+          orewrite (l' + 0=l'). eauto.
+          right; stuck2. rewrite Ldef in H. inv H. get_functional; subst. congruence.
+          right; stuck2. rewrite Ldef in H. inv H. get_functional; subst. congruence.
+        * right; stuck2. rewrite Ldef in H. inv H. eauto.
       + right. stuck.
     - right. stuck.
     - case_eq (omap (exp_eval V) Y); intros; try now (right; stuck).
@@ -196,22 +232,26 @@ Module I.
 
 End I.
 
-Fixpoint labIndices (s:nstmt) (symb: list lab) : status stmt :=
+Definition foo := 3.
+
+Fixpoint labIndices (symb: list var) (s:nstmt) : status stmt :=
   match s with
-    | nstmtLet x e s => sdo s' <- (labIndices s symb); Success (stmtLet x e s')
+    | nstmtLet x e s => sdo s' <- (labIndices symb s); Success (stmtLet x e s')
     | nstmtIf x s1 s2 =>
-      sdo s1' <- (labIndices s1 symb);
-      sdo s2' <- (labIndices s2 symb);
+      sdo s1' <- (labIndices symb s1);
+      sdo s2' <- (labIndices symb s2);
       Success (stmtIf x s1' s2')
     | nstmtApp l Y =>
       sdo f <- option2status (pos symb l 0) "labIndices: Undeclared function" ; Success (stmtApp (LabI f) Y)
     | nstmtReturn x => Success (stmtReturn x)
     | nstmtExtern x f Y s =>
-      sdo s' <- (labIndices s symb); Success (stmtExtern x f Y s')
-    | nstmtFun l Z s1 s2 =>
-      sdo s1' <- labIndices s1 (l::symb);
-      sdo s2' <- labIndices s2 (l::symb);
-      Success (stmtFun Z s1' s2')
+      sdo s' <- (labIndices symb s); Success (stmtExtern x f Y s')
+    | nstmtFun F s2 =>
+      let fl := List.map (fst ∘ fst) F in
+      sdo F' <- smap (fun (fZs:var*params*nstmt) => sdo s <- labIndices (fl ++ symb) (snd fZs);
+                    Success (snd (fst fZs), s)) F;
+      sdo s2' <- labIndices (fl++symb) s2;
+      Success (stmtFun F' s2')
   end.
 
 Definition state_result X (s:X*onv val*nstmt) : option val :=
@@ -239,26 +279,36 @@ Instance statetype_I : StateType I.state := {
                   [ tac | no_step ] ]
         | no_step; tac; simpl in *; eauto ]
   end.
-*)
-Inductive lab_approx : list lab -> env (option I.block) -> list IL.I.block -> Prop :=
+ *)
+
+Inductive lab_approx : list var -> env (option I.block) -> list IL.I.block -> Prop :=
   Lai symb L L'
-    (LEQ: forall f f' s Z Lb,
-             L (counted f) = Some (I.blockI Lb (f',Z,s))
-             -> exists i s',
-                 get L' i (IL.I.blockI Z s')
-                 /\ labIndices s (drop i symb) = Success s'
-                 /\ pos symb f 0 = Some i                                                             /\ lab_approx (drop (S i) symb) (Lb (* [counted f <- Some (I.blockI Lb (f, Z, s))] *)) (drop (S i) L')
-                 /\ (forall l b, Lb (counted l) = Some b -> fst (fst (I.block_F b)) = l)
-                 /\ (forall f i' k, pos (drop (S i) symb) f k = Some i' -> Lb (counted f) <> None)
-                 /\ f = f')
+    (LEQ: forall f f' Lb F,
+            L f = Some (I.blockI Lb F f')
+            ->
+            forall f', f' < length F ->
+                   exists i s' Z s,
+                     get F f' (f,Z,s)
+                     /\ get L' i (IL.I.blockI Z s' f')
+                     /\ labIndices (drop (i - f') symb) s = Success s'
+                     /\ pos symb f 0 = Some i
+                     /\ lab_approx (drop (i + (length F - f')) symb)
+                                  Lb
+                                  (drop (i + (length F - f')) L')
+                     (* /\ (forall l b, Lb (counted l) = Some b -> fst (fst (I.block_F b)) = l) *)
+                     /\ (forall f i' k, pos (drop (i - f') symb) f k = Some i' -> Lb f <> None)
+                     /\ f' <= i /\ f' < length F)
   : lab_approx symb L L'.
+
+
 
 Inductive labIndicesSim : I.state -> IL.I.state -> Prop :=
   | labIndicesSimI (L:env (option I.block)) L' E s s' symb
-    (EQ:labIndices s symb = Success s')
+    (EQ:labIndices symb s = Success s')
     (LA:lab_approx symb L L')
-    (LL:forall l b, L (counted l) = Some b -> fst (fst (I.block_F b)) = l)
-    (EX:forall f i k, pos symb f k = Some i -> L (counted f) <> None)
+(*    (LL:forall l b, L (counted l) = Some b -> fst (fst (I.block_F b)) = l) *)
+    (EX:forall f i k, pos symb f k = Some i -> L f <> None)
+    (SM:forall l blk, L l = Some blk -> I.block_f blk < length (I.block_F blk))
   : labIndicesSim (L, E, s) (L', E, s').
 
 
@@ -297,49 +347,56 @@ Proof.
   - case_eq (exp_eval E e); intros.
     case_eq (val2bool v); intros; one_step; eapply labIndicesSim_sim; econstructor; eauto.
     no_step.
-  - case_eq (L (counted l)); intros.
-    + destruct b as [? [[l0 Z'] s']].
+  - case_eq (L l); intros.
+    + destruct b as [Lb Fb fb].
       eapply option2status_inv in EQ0.
       inv LA.
-      edestruct LEQ as [? [? ?]]; dcr; eauto.
-      assert (x0 = x) by congruence; subst x0.
-      decide (length Z' = length Y).
+      edestruct LEQ as [i [s' [Z s]]]; dcr; eauto.
+      eapply (SM _ _ H).
+      assert (x = i) by congruence. subst x.
+      decide (length Z = length Y).
       case_eq (omap (exp_eval E) Y); intros.
-      one_step. simpl.
+      one_step. orewrite (l + 0 = l). eauto. simpl.
       eapply labIndicesSim_sim.
-      econstructor; eauto. subst l0.
-      * simpl.
-        econstructor. simpl; intros; dcr.
-        lud. inv H7.
-        assert (f = f') by (destruct f, f'; simpl in *; congruence); subst.
-        do 2 eexists. split.
-        eapply drop_get with (n:=0). orewrite (x + 0 = x). eauto.
-        intuition.
-        eapply pos_plus. orewrite (x + 0 = x); eauto.
-        simpl in *. repeat rewrite drop_tl. auto.
-        eapply H6. simpl in H9. rewrite drop_tl in H9. eapply H9. eauto.
-        inv H4.
-        edestruct (LEQ0); eauto. destruct H10; dcr.
-        eexists (S x0), x2. split; eauto using get.
-        eapply drop_get. orewrite (x + S x0 = S x + x0). eapply get_drop. eauto.
-        repeat rewrite drop_tl in *. repeat rewrite drop_drop in *.
-        orewrite (S x0 + x = x0 + S x); eauto.
-        repeat (split; eauto).
-        exploit pos_drop_eq; [eapply H2|].
-        rewrite X. unfold pos; fold pos. destruct if. congruence.
-        rewrite drop_tl. eapply (pos_add 1); eauto.
-      * subst l0. intros. lud. inv H7.
-        assert (l = l0) by (destruct l, l0; simpl in *; congruence); subst.                 simpl; eauto.
-        eapply H5; eauto.
-      * subst l. intros. lud. congruence. eapply H6; eauto.
-        exploit pos_drop_eq; [eapply H2|].
-        rewrite X in H7. unfold pos in H7; fold pos in H7.
-        destruct if in H7. destruct f, l0; simpl in *; congruence.
-        simpl. rewrite <- drop_tl. eauto.
-      * subst l. no_step.
-      * subst. no_step.
-        edestruct LEQ as [? [? ?]]; eauto; dcr.
-        get_functional; subst; simpl in *. congruence.
+      econstructor; eauto.
+      * econstructor. simpl; intros; dcr. {
+        decide (f ∈ of_list (List.map (fst ∘ fst) Fb)).
+        - eapply update_with_list_lookup_in_list in i0. dcr.
+          erewrite H13 in H9. subst. invc H15. inv_map H11.
+          unfold I.mkBlocks, I.mkBlock in H9.
+          inv_mapi H9. inv_map H12.
+          destruct x1 as [[? ?] ?]. unfold comp in *; simpl in *.
+          eexists f'. do 3 eexists; split; eauto. split.
+          eapply drop_get.
+          exfalso; admit. exfalso; admit. admit.
+        - erewrite (update_with_list_no_update _ _ _ n) in H9; eauto.
+          inv H4.
+          exploit LEQ0; eauto; dcr; clear LEQ0.
+          eexists (x + length Fb).
+          do 3 eexists; split; eauto.
+          split; eauto.
+          eapply drop_get. eapply get_drop in H11.
+          orewrite (i - fb + (x + length Fb) = i + (length Fb - fb) + x). eauto.
+          split. rewrite drop_drop. rewrite drop_drop in H12.
+          orewrite (x + length Fb - f' + (i - fb) = x - f' + (i + (length Fb - fb))); eauto.
+          split.
+          admit.
+          split. repeat rewrite drop_drop in *.
+          orewrite (x + length Fb + (length F - f') + (i - fb) = x + (length F - f') + (i + (length Fb - fb))). eauto.
+          repeat split; try omega.
+          intros. rewrite drop_drop in *.
+          orewrite (x + length Fb - f' + (i - fb) = x - f' + (i + (length Fb - fb))) in H17; eauto.
+        }
+      * intros.
+        decide (f ∈ of_list (List.map (fst ∘ fst) Fb)).
+        eapply update_with_list_lookup_in_list in i1. dcr.
+        erewrite H12. inv_map H10. congruence. repeat rewrite map_length.
+        unfold I.mkBlocks, I.mkBlocks, mapi. rewrite mapi_length. reflexivity.
+        erewrite (update_with_list_no_update _ _ _ n); eauto.
+      * intros. no_step.
+      * no_step.
+        rewrite Ldef in H. inv H. simpl in *. repeat get_functional; subst. eauto.
+        repeat get_functional; subst. eauto.
     + eapply option2status_inv in EQ0. exfalso. eapply EX; eauto.
   - no_step.
   - case_eq (omap (exp_eval E) Y); intros.
@@ -352,22 +409,68 @@ Proof.
     + no_step.
   - one_step. eapply labIndicesSim_sim. econstructor; eauto.
     econstructor. intros.
-    + lud.
-      * inv H. do 2 eexists.
-        split. econstructor. intuition. unfold pos; fold pos.
-        destruct if; eauto. cbv in n; destruct f, f'; simpl in *; congruence.
-        destruct f, f'; simpl in *; congruence.
-      * inv LA. edestruct LEQ; eauto. destruct H2.
-        eexists (S x1),x2. dcr. split; eauto using get.
-        split; eauto. split; eauto.
-        unfold pos; fold pos. destruct if; eauto.
-                                         congruence.
-        intros. eapply (pos_add 1); eauto.
-    + intros. lud; eauto.
-      inv H; eauto. destruct l, l0; simpl in *; congruence; eauto.
-    + intros. lud. congruence.
-      unfold pos in H; fold pos in H.
-      destruct if in H. congruence. eapply EX; eauto.
+    + decide (f ∈ of_list (List.map (fst ∘ fst) F)).
+      * eapply update_with_list_lookup_in_list in i. dcr.
+        erewrite H2 in H. subst. invc H4. clear H2.
+        inv_map H1. inv_map H0.
+        unfold I.mkBlocks, I.mkBlock in *. inv_mapi H3.
+        repeat get_functional; subst.
+        destruct x3 as [[fb Zb] sb]; unfold comp in *; simpl in *.
+        pose proof EQ0 as SM.
+        eapply smap_spec in EQ0; eauto. destruct EQ0; eauto; dcr. monadS_inv H2.
+        simpl in *.
+        do 4 eexists; split; eauto. instantiate (1:=f').
+        split; eauto. eapply get_app.
+        unfold IL.I.mkBlocks. instantiate (1:=x2). admit.
+        split; eauto. orewrite (f' - f' = 0); simpl. eauto.
+        split; eauto. admit.
+        split; eauto.
+        exploit (get_length H4); eauto.
+        orewrite (f' + (length F0 - f') = length F0 + 0); simpl.
+        assert (length F0 = length (List.map (fun x1 : var * params * nstmt => fst (fst x1)) F0)).
+        rewrite map_length; eauto. rewrite H at 1.
+        rewrite drop_app.
+        assert (length F0 = length (IL.I.mkBlocks x)).
+        unfold IL.I.mkBlocks, mapi.
+        rewrite mapi_length; eauto. eapply smap_length in SM; eauto.
+        rewrite H2. rewrite drop_app. eauto.
+        split; eauto.
+        orewrite (f' - f' = 0). simpl. admit.
+        repeat rewrite map_length. unfold I.mkBlocks, mapi.
+        rewrite mapi_length; eauto.
+      * erewrite (update_with_list_no_update _ _ _ n) in H.
+        inv LA. exploit LEQ; eauto; clear LEQ. dcr.
+        exploit smap_length; eauto.
+        assert (length (IL.I.mkBlocks x) = length (List.map (fst ∘ fst) F)). {
+          rewrite map_length. unfold IL.I.mkBlocks, mapi.
+          rewrite mapi_length; eauto.
+        }
+        do 4 eexists; split; eauto.
+        split. eapply get_shift; eauto.
+        split. orewrite ((length (IL.I.mkBlocks x) + x1 - f' =
+                          length (IL.I.mkBlocks x) + (x1 - f'))).
+        rewrite H6. rewrite drop_app. eauto.
+        split; eauto. rewrite pos_app_not_in; eauto.
+        rewrite H6. eapply pos_add; eauto.
+        split. orewrite (length (IL.I.mkBlocks x) + x1 + (length F0 - f') =
+                         length (IL.I.mkBlocks x) + (x1 + (length F0 - f'))).
+        rewrite H6 at 1. repeat rewrite drop_app. eauto.
+        split; eauto.
+        intros.
+        orewrite ((length (IL.I.mkBlocks x) + x1 - f' =
+                   length (IL.I.mkBlocks x) + (x1 - f'))) in H8.
+        rewrite H6 in H8.
+        rewrite drop_app in H8. eauto.
+        omega.
+    + intros.
+      decide (f ∈ of_list (List.map (fst ∘ fst) F)).
+      * pose proof (pos_app_in k _ symb i0); eauto. erewrite H0 in H. clear H0.
+        eapply update_with_list_lookup_in_list in i0. dcr.
+        erewrite H2. invc H4. inv_map H0. congruence.
+        repeat rewrite map_length. unfold I.mkBlocks, mapi. rewrite mapi_length; eauto.
+      * erewrite (update_with_list_no_update _ _ _ n).
+        pose proof (pos_app_not_in k _ symb n); eauto. erewrite H0 in H. clear H0.
+        eauto.
 Qed.
 
 (*
